Added new definitions and theorems for various bit-vector "saturation" operations.
These operations return maximal or minimal values instead of, e.g.,
overflowing (wrapping).  For example:

|- signed_saturate_add 100w 50w = 127w: thm

Also added a new configuration option for printing word literals as 2's
complement values.  For example:

> set_trace "word pp as 2's comp" 1;
> ``253w:word8``;
val it = ``-3w``: term

Be warned that this term is actually ``n2w 253``, it's just being printed as
``word_2comp (n2w 3)``.

This printing mode is useful when checking the veracity of machine arithmetic.
For example:

> EVAL ``signed_saturate_sub 226w 100w : word8``;
val it = |- signed_saturate_sub -30w 100w = -128w: thm

src/integer/integer_wordSyntax.sig
@@ -2,16 +2,56 @@ signature integer_wordSyntax = sig
 
   include Abbrev
 
-  val i2w_tm   : term
-  val w2i_tm   : term
+  val i2w_tm                 : term
+  val w2i_tm                 : term
+  val int_min_tm             : term
+  val int_max_tm             : term
+  val uint_max_tm            : term
+  val saturate_i2sw_tm       : term
+  val saturate_i2w_tm        : term
+  val saturate_sw2sw_tm      : term
+  val saturate_sw2w_tm       : term
+  val saturate_w2sw_tm       : term
+  val signed_saturate_add_tm : term
+  val signed_saturate_sub_tm : term
 
-  val mk_i2w   : term * hol_type -> term
-  val mk_w2i   : term -> term
+  val mk_i2w                 : term * hol_type -> term
+  val mk_w2i                 : term -> term
+  val mk_int_min             : hol_type -> term
+  val mk_int_max             : hol_type -> term
+  val mk_uint_max            : hol_type -> term
+  val mk_saturate_i2sw       : term * hol_type -> term
+  val mk_saturate_i2w        : term * hol_type -> term
+  val mk_saturate_sw2sw      : term * hol_type -> term
+  val mk_saturate_sw2w       : term * hol_type -> term
+  val mk_saturate_w2sw       : term * hol_type -> term
+  val mk_signed_saturate_add : term * term -> term
+  val mk_signed_saturate_sub : term * term -> term
 
-  val dest_i2w : term -> term
-  val dest_w2i : term -> term
+  val dest_i2w                 : term -> term
+  val dest_w2i                 : term -> term
+  val dest_int_min             : term -> hol_type
+  val dest_int_max             : term -> hol_type
+  val dest_uint_max            : term -> hol_type
+  val dest_saturate_i2sw       : term -> term * hol_type
+  val dest_saturate_i2w        : term -> term * hol_type
+  val dest_saturate_sw2sw      : term -> term * hol_type
+  val dest_saturate_sw2w       : term -> term * hol_type
+  val dest_saturate_w2sw       : term -> term * hol_type
+  val dest_signed_saturate_add : term -> term * term
+  val dest_signed_saturate_sub : term -> term * term
 
-  val is_i2w   : term -> bool
-  val is_w2i   : term -> bool
+  val is_i2w                 : term -> bool
+  val is_w2i                 : term -> bool
+  val is_int_min             : term -> bool
+  val is_int_max             : term -> bool
+  val is_uint_max            : term -> bool
+  val is_saturate_i2sw       : term -> bool
+  val is_saturate_i2w        : term -> bool
+  val is_saturate_sw2sw      : term -> bool
+  val is_saturate_sw2w       : term -> bool
+  val is_saturate_w2sw       : term -> bool
+  val is_signed_saturate_add : term -> bool
+  val is_signed_saturate_sub : term -> bool
 
 end
