src/integer/integer_wordSyntax.sml
@@ -2,27 +2,162 @@ structure integer_wordSyntax :> integer_wordSyntax =
 struct
 
 open HolKernel boolLib;
-open integer_wordTheory;
+open wordsSyntax integer_wordTheory;
 
-val ERR = mk_HOL_ERR "integer_wordSyntax";
+val ERR = Feedback.mk_HOL_ERR "integer_wordSyntax";
 
-fun mk_integer_word_const s =  prim_mk_const{Name = s, Thy = "integer_word"};
+(*---------------------------------------------------------------------------
+  Terms
+  ---------------------------------------------------------------------------*)
+
+fun mk_integer_word_const s =
+   Term.prim_mk_const {Name = s, Thy = "integer_word"};
 
 val w2i_tm = mk_integer_word_const "w2i";
 val i2w_tm = mk_integer_word_const "i2w";
 
+val int_min_tm  = mk_integer_word_const "INT_MIN";
+val int_max_tm  = mk_integer_word_const "INT_MAX";
+val uint_max_tm = mk_integer_word_const "UINT_MAX";
+
+val saturate_i2sw_tm  = mk_integer_word_const "saturate_i2sw";
+val saturate_i2w_tm   = mk_integer_word_const "saturate_i2w";
+val saturate_sw2sw_tm = mk_integer_word_const "saturate_sw2sw";
+val saturate_sw2w_tm  = mk_integer_word_const "saturate_sw2w";
+val saturate_w2sw_tm  = mk_integer_word_const "saturate_w2sw";
+val signed_saturate_add_tm = mk_integer_word_const "signed_saturate_add";
+val signed_saturate_sub_tm = mk_integer_word_const "signed_saturate_sub";
+
+(*---------------------------------------------------------------------------
+  Constructors
+  ---------------------------------------------------------------------------*)
+
 fun mk_w2i w =
-  mk_comb (inst[alpha |-> wordsSyntax.dim_of w] w2i_tm,w)
+  Term.mk_comb (Term.inst [Type.alpha |-> wordsSyntax.dim_of w] w2i_tm, w)
   handle HOL_ERR _ => raise ERR "mk_word_w2i" "";
 
-fun mk_i2w (n,ty) =
-  mk_comb (inst[alpha |-> ty] i2w_tm,n)
+fun mk_i2w (n, ty) =
+  Term.mk_comb (Term.inst [Type.alpha |-> ty] i2w_tm, n)
   handle HOL_ERR _ => raise ERR "mk_word_i2w" "";
 
-val dest_i2w = dest_monop i2w_tm (ERR "dest_i2w" "");
-val dest_w2i = dest_monop w2i_tm (ERR "dest_i2w" "");
+fun mk_uint_max ty =
+  Term.mk_comb
+    (Term.inst [Type.alpha |-> ty] uint_max_tm,
+     boolSyntax.mk_itself ty)
+  handle HOL_ERR _ => raise ERR "mk_uint_max" "";
+
+fun mk_int_min ty =
+  Term.mk_comb
+    (Term.inst [Type.alpha |-> ty] int_min_tm,
+     boolSyntax.mk_itself ty)
+  handle HOL_ERR _ => raise ERR "mk_int_min" "";
+
+fun mk_int_max ty =
+  Term.mk_comb
+    (Term.inst [Type.alpha |-> ty] int_max_tm,
+     boolSyntax.mk_itself ty)
+  handle HOL_ERR _ => raise ERR "mk_int_max" "";
+
+fun mk_saturate_i2sw (n, ty) =
+  Term.mk_comb (Term.inst [Type.alpha |-> ty] saturate_i2sw_tm, n)
+  handle HOL_ERR _ => raise ERR "mk_saturate_i2sw" "";
+
+fun mk_saturate_i2w (n, ty) =
+  Term.mk_comb (Term.inst [Type.alpha |-> ty] saturate_i2w_tm, n)
+  handle HOL_ERR _ => raise ERR "mk_saturate_i2w" "";
+
+fun mk_saturate_sw2sw (w, ty) =
+  Term.mk_comb
+    (Term.inst
+       [Type.alpha |-> wordsSyntax.dim_of w, Type.beta |-> ty]
+       saturate_sw2sw_tm, w)
+  handle HOL_ERR _ => raise ERR "mk_saturate_sw2sw" "";
+
+fun mk_saturate_sw2w (w, ty) =
+  Term.mk_comb
+    (Term.inst
+       [Type.alpha |-> wordsSyntax.dim_of w, Type.beta |-> ty]
+       saturate_sw2w_tm, w)
+  handle HOL_ERR _ => raise ERR "mk_saturate_sw2w" "";
+
+fun mk_saturate_w2sw (w, ty) =
+  Term.mk_comb
+    (Term.inst
+       [Type.alpha |-> wordsSyntax.dim_of w, Type.beta |-> ty]
+       saturate_w2sw_tm, w)
+  handle HOL_ERR _ => raise ERR "mk_saturate_w2sw" "";
+
+fun mk_signed_saturate_add (w1, w2) =
+  list_mk_comb (inst [alpha |-> dim_of w1] signed_saturate_add_tm, [w1, w2])
+  handle HOL_ERR _ => raise ERR "mk_signed_saturate_add" "";
+
+fun mk_signed_saturate_sub (w1, w2) =
+  list_mk_comb (inst [alpha |-> dim_of w1] signed_saturate_sub_tm, [w1, w2])
+  handle HOL_ERR _ => raise ERR "mk_signed_saturate_sub" "";
+
+(*---------------------------------------------------------------------------
+  Destructorss
+  ---------------------------------------------------------------------------*)
+
+val dest_i2w = HolKernel.dest_monop i2w_tm (ERR "dest_i2w" "");
+val dest_w2i = HolKernel.dest_monop w2i_tm (ERR "dest_i2w" "");
+
+val dest_uint_max =
+  boolSyntax.dest_itself o
+  HolKernel.dest_monop uint_max_tm (ERR "dest_uint_max" "");
+
+val dest_int_min =
+  boolSyntax.dest_itself o
+  HolKernel.dest_monop int_min_tm (ERR "dest_int_min" "");
+
+val dest_int_max =
+  boolSyntax.dest_itself o
+  HolKernel.dest_monop int_max_tm (ERR "dest_int_max" "");
+
+fun dest_saturate_i2sw M =
+  (dest_monop saturate_i2sw_tm (ERR "dest_saturate_i2sw" "") M,
+   wordsSyntax.dim_of M);
+
+fun dest_saturate_i2w M =
+  (dest_monop saturate_i2w_tm (ERR "dest_saturate_i2w" "") M,
+   wordsSyntax.dim_of M);
+
+fun dest_saturate_sw2sw M =
+  (dest_monop saturate_sw2sw_tm (ERR "dest_saturate_sw2sw" "") M,
+   wordsSyntax.dim_of M);
+
+fun dest_saturate_sw2w M =
+  (dest_monop saturate_sw2w_tm (ERR "dest_saturate_sw2s" "") M,
+   wordsSyntax.dim_of M);
+
+fun dest_saturate_w2sw M =
+  (dest_monop saturate_w2sw_tm (ERR "dest_saturate_w2sw" "") M,
+   wordsSyntax.dim_of M);
+
+val dest_signed_saturate_add =
+  dest_binop signed_saturate_add_tm (ERR "dest_signed_saturate_add" "");
+
+val dest_signed_saturate_sub =
+  dest_binop signed_saturate_sub_tm (ERR "dest_signed_saturate_sub" "");
+
+(*---------------------------------------------------------------------------
+  Discriminators
+  ---------------------------------------------------------------------------*)
 
 val is_i2w = Lib.can dest_i2w;
 val is_w2i = Lib.can dest_w2i;
+
+val is_uint_max = Lib.can dest_uint_max;
+val is_int_min  = Lib.can dest_int_min;
+val is_int_max  = Lib.can dest_int_max;
+
+val is_saturate_i2sw  = Lib.can dest_saturate_i2sw;
+val is_saturate_i2w   = Lib.can dest_saturate_i2w;
+val is_saturate_sw2sw = Lib.can dest_saturate_sw2sw;
+val is_saturate_sw2w  = Lib.can dest_saturate_sw2w;
+val is_saturate_w2sw  = Lib.can dest_saturate_w2sw;
+
+val is_signed_saturate_add = Lib.can dest_signed_saturate_add
+val is_signed_saturate_sub = Lib.can dest_signed_saturate_sub
 
 end
